\documentclass[journal,12pt,two column]{IEEEtran}
\usepackage{setspace}
\usepackage{listings}
%\singlespacing
%\usepackage{gensymb}
\usepackage{enumitem}
\usepackage[cmex10]{amsmath}
\usepackage{amssymb}
\bibliographystyle{IEEEtran}
%\usepackage{tfrupee}
\usepackage{amsthm}
\usepackage[utf8]{inputenc}
\title{Assignment 2 (ICSE 2018)}
\author{Nitya Seshagiri Bhamidipaty (cs21btech11041)}
\providecommand{\brak}[1]{\ensuremath{\left(#1\right)}}
\newcommand{\solution}{\noindent \textbf{Solution: }}
\begin{document}
\maketitle
\begin{enumerate}
\item[\textbf{13 (a)}] Evaluate: $\int\frac{x-1}{\sqrt{x^2-x}}dx$\\
\solution 
\begin{align}
    \frac{x-1}{\sqrt{x^2-x}} %&= \frac{\frac{1}{2}(2x-1) - \frac{1}{2}}{\sqrt{x^2-x}}
    &= \frac{1}{2}\frac{2x-1}{\sqrt{x^2-x}} - \frac{1}{2}\frac{1}{\sqrt{x^2-x}}
\end{align}
Integrating both sides
\begin{multline}
\int \frac{x-1}{\sqrt{x^2-x}} \, dx = \frac{1}{2}\int\frac{2x-1}{\sqrt{x^2-x}} \, dx \\
    -  \frac{1}{2}\int\frac{1}{\sqrt{x^2-x}} \, dx
    \label{eq:3}
\end{multline}
Let $t = x^2-x$
\begin{align}
    dt = (2x - 1)dx
    \\
    \int\frac{2x-1}{\sqrt{x^2-x}} \, dx &= \int\frac{dt}{\sqrt{t}}
    \\
    &= 2\sqrt{t}+C
    \\
    &= 2\sqrt{x^2-x}+C
    \label{eq:7}
    %& \brak{\frac{x^2+x}{x}}
\end{align}
Also let $u = x - \frac{1}{2}$

\begin{align}
    du = dx\\
    \int\frac{1}{\sqrt{x^2-x}} \, dx &= \int\frac{1}{\sqrt{\brak{x-\frac{1}{2}}^2 - \frac{1}{4}}} \, dx
    \\
    &=\int\frac{1}{\sqrt{u^2 - \brak{\frac{1}{2}}^2}} \, du
    \\
    &= \ln \left|u + \sqrt{u^2-\brak{\frac{1}{2}}^2}\right| + C
    \\
    &= \ln \left|x - \frac{1}{2} + \sqrt{x^2-x}\right|+C
    \label{eq:12}
\end{align}
From eq\eqref{eq:3}, eq\eqref{eq:7}, eq\eqref{eq:12} we get 
\begin{multline}
    \int\frac{x-1}{\sqrt{x^2-x}} \, dx = \frac{1}{2}\times2\sqrt{x^2-x} -\\
    \frac{1}{2} \ln \left|x - \frac{1}{2} + \sqrt{x^2-x}\right| +C
\end{multline}
Hence,
\begin{multline}
    \int \frac{x-1}{\sqrt{x^2-x}} \, dx = \sqrt{x^2-x} \\- \frac{1}{2}\ln \left|2x-1 + \sqrt{4x^2-4x}\right| + C
\end{multline}

\end{enumerate}
\end{document}